WIP, experiments with checker

Experiments/ProofChecking/RangeArray.lean
@@ -706,6 +706,10 @@ theorem append_empty (A : RangeArray α) : A.append Array.empty = A.clear.commit
   simp [append, Array.empty, commit]
 
 @[simp]
+theorem append_empty' (A : RangeArray α) : A.append #[] = A.clear.commit := by
+  simp [append, Array.empty, commit]
+
+@[simp]
 theorem append_nil (A : RangeArray α) : A.append { data := [] } = A.clear.commit :=
   append_empty A
 
@@ -716,24 +720,20 @@ theorem append_eq_append'_aux :
   have ⟨L⟩ := arr
   rw [append']
   induction' L with x xs ih generalizing A
-  · simp [commit, LeanColls.size]; rfl
+  · simp [commit, LeanColls.size]
   · rw [foldl_cons]
     rw [ih (push A x)]
     simp [push, Seq.snoc]
     constructor
     · have : A.data.push x = A.data ++ #[x] := rfl
       rw [this]
-      rw [Array.append_assoc]
-      congr
-      -- CC: Simple array fact
-      sorry
+      rw [Array.append_assoc, Array.singleton_append_data_eq_cons]
     · simp [LeanColls.size, succ_eq_add_one]
       rw [add_assoc, add_comm 1 (List.length xs)]
 
 theorem append_eq_append' : A.append arr = (A.clear).append' arr := by
   rw [append, append_eq_append'_aux A.clear arr]
 
--- CC: This might be unneeded?
 @[simp]
 theorem append_indexes : (A.append arr).indexes = Seq.snoc A.indexes (A.dsize : Int) := by
   rw [append_eq_append']
@@ -777,17 +777,19 @@ theorem rsize_append_lt {A : RangeArray α} {i : Nat} (hi : i < A.size) (arr : A
   simp [append', hi, lt_succ_of_lt hi, size]
   simp [rsize, rsizeFin, index, indexFin, size, hi, lt_succ_of_lt hi, Seq.get_snoc]
   split <;> rename _ => hi'
-  · stop
-    congr 1
-  · stop
-    have := le_antisymm (Nat.succ_le_of_lt hi) (not_lt.mp hi')
+  · rfl
+  · have := le_antisymm (Nat.succ_le_of_lt hi) (not_lt.mp hi')
     rw [succ_eq_add_one] at this
     simp [this]
 
+@[simp]
 theorem rsize_append_eq : (A.append arr).rsize A.size = Size.size arr := by
-  simp [rsize, rsizeFin]
-  stop
-  done
+  rw [append_eq_append']
+  simp [rsize, size, append', rsizeFin, dsize]
+  rw [indexFin_eq_index]
+  simp
+  conv => lhs; lhs; rw [Nat.add_comm]
+  simp [index, indexFin, size]
 
 @[simp]
 theorem usize_append (arr : Array α) : (A.append arr).usize = 0 := by
@@ -800,6 +802,7 @@ theorem isDeleted_append_lt {A : RangeArray α} {i : Nat} (hi : i < A.size) (arr
   simp [append', hi, lt_succ_of_lt hi, size]
   simp [isDeleted, isDeletedFin, hi, lt_succ_of_lt hi, Seq.get_snoc, size]
 
+@[simp]
 theorem isDeleted_append_eq : (A.append arr).isDeleted A.size = false := by
   rw [append_eq_append']
   simp [append', isDeleted, isDeletedFin, size, Seq.get_snoc]
@@ -867,6 +870,14 @@ theorem get_clear_ge {A : RangeArray α} {i : Nat} (hi : i ≥ A.dsize) :
     exact absurd (lt_of_lt_of_le h_con this) (not_lt_of_ge hi)
   · simp [LeanColls.size, hi]
 
+theorem get_commit_lt {A : RangeArray α} {i : Nat} (hi : i < Size.size A.data) :
+    (A.commit).get i = A.get i := by
+  simp [get, getFin, commit, hi, usize]
+
+theorem get_commit_lt_usize {A : RangeArray α} {i : Nat} (hi : i < A.usize) :
+    (A.commit).get (A.dsize + i) = A.get (A.dsize + i) := by
+  simp [get, getFin, commit, hi, usize]
+
 /- theorem get_append_lt {A : RangeArray α} {i : Nat} (hi : i < A.dsize) (arr : Array α) :
     (A.append arr).get i = A.get i := by -/
 
@@ -887,18 +898,25 @@ theorem indexFin_add_rsizeFin_le_size {A : RangeArray α}
     exact A.h_size
     exact A.h_indexes hi
 
-theorem index_add_offset_in_range {A : RangeArray α}
+theorem indexFin_add_offset_lt_size {A : RangeArray α}
       (i : Fin A.size) (offset : Fin (A.rsizeFin i)) :
     A.indexFin i + offset.val < Size.size A.data := by
   have := indexFin_add_rsizeFin_le_size i
   apply lt_of_lt_of_le (by omega) this
+
+theorem index_add_offset_lt_size {A : RangeArray α} {i offset : Nat}
+      (hi : i < A.size) (ho : offset < A.rsize i) :
+    A.index i + offset < Size.size A.data := by
+  have := indexFin_add_offset_lt_size ⟨i, hi⟩ ⟨offset, by rw [rsizeFin_eq_rsize]; exact ho⟩
+  rw [indexFin_eq_index] at this
+  exact this
 
 /-! # oget and uget -/
 
 @[inline, always_inline]
 def ogetFin {A : RangeArray α} (i : Fin A.size) (offset : Fin (A.rsizeFin i)) : α :=
   A.getFin ⟨A.indexFin i + offset.val,
-      index_add_offset_in_range i offset⟩
+      indexFin_add_offset_lt_size i offset⟩
 
 @[inline, always_inline]
 def oget (i offset : Nat) : α :=
@@ -918,7 +936,7 @@ theorem ogetFin_eq_oget' (i : Fin A.size) (offset : Fin (A.rsizeFin i)) :
 
 theorem ogetFin_eq_getFin {i offset : Nat} (hi : i < A.size) (ho : offset < A.rsizeFin ⟨i, hi⟩) :
     A.ogetFin ⟨i, hi⟩ ⟨offset, ho⟩ =
-      A.getFin ⟨A.indexFin ⟨i, hi⟩ + offset, index_add_offset_in_range ⟨i, hi⟩ ⟨offset, ho⟩⟩ := by
+      A.getFin ⟨A.indexFin ⟨i, hi⟩ + offset, indexFin_add_offset_lt_size ⟨_, hi⟩ ⟨_, ho⟩⟩ := by
   simp [ogetFin]
 
 @[inline, always_inline]
@@ -954,41 +972,55 @@ theorem oget_push (A : RangeArray α) (i offset : Nat) (v : α) :
 
 theorem oget_commit_lt {A : RangeArray α} {i offset : Nat} (hi : i < A.size) (ho : offset < A.rsize i) :
     (A.commit).oget i offset = A.oget i offset := by
-  simp [oget]
-  stop
-  split <;> rename _ => hi
-  · split <;> rename _ => ho
-    · rw [ogetFin]
-      simp [commit, Seq.get_snoc, indexFin]
-      done
-    done
-  done
+  simp [oget, ogetFin, hi, lt_succ_of_lt hi]
+  simp_rw [rsizeFin_eq_rsize, getFin_eq_get, indexFin_eq_index]
+  simp [ho, index_commit_lt hi]
+  apply get_commit_lt
+  exact index_add_offset_lt_size hi ho
 
 theorem oget_commit_eq {A : RangeArray α} {offset : Nat} (ho : offset < A.usize) :
     (A.commit).oget A.size offset = A.uget offset := by
-  stop
-  done
+  simp [oget, ogetFin, uget, ugetFin, ho]
+  simp_rw [indexFin_eq_index, getFin_eq_get]
+  simp
+  apply get_commit_lt
+  simp [usize] at ho
+  omega
 
 theorem oget_delete_ne (A : RangeArray α) {i j offset : Nat} (hij : i ≠ j) :
     (A.delete i).oget j offset = A.oget j offset := by
-  stop
-  done
+  simp [delete]
+  split <;> rename _ => hi <;> try rfl
+  simp [oget, ogetFin]
+  split <;> rename _ => hj <;> try rfl
+  simp_rw [rsizeFin_eq_rsize, deleteFin_eq_delete]
+  simp [rsize_delete_ne hij]
+  split <;> rename _ => ho <;> try rfl
+  simp [getFin, deleteFin, indexFin, Seq.get_set, hij]
 
 theorem uget_push_lt {A : RangeArray α} {i : Nat} (hi : i < A.usize) (v : α) :
     (A.push v).uget i = A.uget i := by
-  simp [uget]
-  stop
-  done
+  simp [uget, ugetFin, hi, lt_succ_of_lt hi]
+  simp_rw [getFin_eq_get]
+  apply get_push_lt
+  simp [usize] at hi
+  omega
 
 @[simp]
 theorem uget_push_eq : (A.push v).uget A.usize = v := by
-  stop
-  done
+  simp [uget, ugetFin]
+  rw [getFin_eq_get]
+  simp [usize]
+  rw [← Nat.add_sub_assoc A.h_size, Nat.add_comm, Nat.add_sub_cancel]
+  exact get_push_eq _ _
 
-theorem uget_delete {A : RangeArray α} {i : Nat} (hi : i < A.usize) (j : Nat) :
+@[simp]
+theorem uget_delete (A : RangeArray α) (i j : Nat) :
     (A.delete j).uget i = A.uget i := by
-  stop
-  done
+  simp [delete]
+  split <;> rfl
+
+/-! # models -/
 
 structure models (R : RangeArray α) (Ls : List (Option (List α))) (L : List α) : Prop where
   (h_size₁ : R.size = Size.size Ls)
@@ -1004,8 +1036,9 @@ structure models (R : RangeArray α) (Ls : List (Option (List α))) (L : List α
   (h_uncommitted : ∀ {i : Nat} (hi : i < Size.size L),
       R.uget i = Seq.get L ⟨i, hi⟩)
 
-theorem get_eq_some_of_models_of_not_deleted {R : RangeArray α} {Ls : List (Option (List α))} {L : List α}
-    (h_models : models R Ls L) {i : Nat} :
+variable {R : RangeArray α} {Ls : List (Option (List α))} {L : List α} (h_models : models R Ls L)
+
+theorem get_eq_some_of_models_of_not_deleted {i : Nat} :
     R.isDeleted i = false → (hi : i < Size.size Ls) ×' ∃ sL, Seq.get Ls ⟨i, hi⟩ = some sL := by
   intro h_del
   by_cases hi : i < Size.size Ls
@@ -1020,19 +1053,15 @@ theorem get_eq_some_of_models_of_not_deleted {R : RangeArray α} {Ls : List (Opt
 theorem models_empty (size : Nat) : models (empty size) ([] : List (Option (List α))) [] := by
   constructor <;> simp
 
-theorem models_push : models A Ls L → ∀ (v : α), models (A.push v) Ls (Seq.snoc L v) := by
-  intro h_models v
+theorem models_push : ∀ (v : α), models (R.push v) Ls (Seq.snoc L v) := by
+  intro v
   constructor
   · simp [h_models.h_size₁]
   · simp [h_models.h_size₂]
   · refine h_models.h_some
-  · intro i hi sL hsL
-    exact h_models.h_sizes hi hsL
+  · refine h_models.h_sizes
   · intro i hi sL hsL j hj
-    have hi₁ := h_models.h_size₁.symm ▸ hi
-    have hj₁ := (h_models.h_sizes hi hsL).symm ▸ hj
-    rw [oget_push_lt hi₁ hj₁ v]
-    exact h_models.h_agree hi hsL hj
+    simp [h_models.h_agree hi hsL hj]
   · intro i hi
     have hi₁ := hi
     rw [Seq.size_snoc, ← h_models.h_size₂] at hi₁
@@ -1050,8 +1079,7 @@ theorem models_push : models A Ls L → ∀ (v : α), models (A.push v) Ls (Seq.
         rw [this] at hi'
         exact absurd hi' (not_lt.mpr (le_refl _))
 
-theorem models_commit : models A Ls L → models (A.commit) (Seq.snoc Ls (some L)) [] := by
-  intro h_models
+theorem models_commit : models (R.commit) (Seq.snoc Ls (some L)) [] := by
   constructor
   · simp [h_models.h_size₁]
   · simp [h_models.h_size₂]
@@ -1099,16 +1127,16 @@ theorem models_commit : models A Ls L → models (A.commit) (Seq.snoc Ls (some L
       exact h_models.h_agree hi₂ hsL hj
   · simp
 
-theorem models_delete : models A Ls L → ∀ {i : Nat} (hi : i < Size.size Ls),
-    models (A.delete i) (Seq.set Ls ⟨i, hi⟩ none) L := by
-  intro h_models i hi
+theorem models_delete : ∀ {i : Nat} (hi : i < Size.size Ls),
+    models (R.delete i) (Seq.set Ls ⟨i, hi⟩ none) L := by
+  intro i hi
   constructor
   · simp [h_models.h_size₁]
   · simp [h_models.h_size₂]
   · intro j hj
     by_cases hij : i = j
     · simp [hij]
-    · rw [isDeleted_delete_ne A hij]
+    · rw [isDeleted_delete_ne R hij]
       simp [Seq.get_set, hij, -eq_iff_iff]
       simp at hj
       exact h_models.h_some hj
@@ -1117,9 +1145,7 @@ theorem models_delete : models A Ls L → ∀ {i : Nat} (hi : i < Size.size Ls),
     · simp [Seq.get_set, hij] at hsL
     · simp [Seq.get_set, hij] at hsL
       simp at hj
-      have := h_models.h_some hj
-      simp [hsL] at this
-      rw [rsize_delete_ne hij this]
+      rw [rsize_delete_ne hij]
       exact h_models.h_sizes hj hsL
   · intro j hj sL hsL k hk
     by_cases hij : i = j
@@ -1127,30 +1153,18 @@ theorem models_delete : models A Ls L → ∀ {i : Nat} (hi : i < Size.size Ls),
     simp at hj
     have := h_models.h_some hj
     simp [hsL] at this
-    rw [oget_delete_ne A hij]
+    rw [oget_delete_ne R hij]
     exact h_models.h_agree hj hsL hk
   · intro j hj
-    simp [uget_delete (h_models.h_size₂.symm ▸ hj)]
+    simp [uget_delete]
     exact h_models.h_uncommitted hj
 
-theorem exists_model (A : RangeArray α) :
-    ∃ (Ls : List (Option (List α))) (L : List α), models A Ls L := by
-  rcases A with ⟨data, indexes, dataSize, _, h_size, h_dataSize_empty, h_indexes, h_indexes_inc⟩
-  rcases data with ⟨data⟩
-  rcases indexes with ⟨indexes⟩
-  -- CC: We might want to induct instead on indexes.size and "go backwards"
-  induction' indexes with i is ih generalizing data
-  · use [], data
-    simp [LeanColls.size] at h_dataSize_empty
-    constructor <;> try simp [size] <;> try rfl
-    · simp [usize, dsize, h_dataSize_empty]; rfl
-    · intro i hi
-      stop
-      done
+-- CC: Which direction does this theorem need to be in?
+/- theorem exists_model (A : RangeArray α) :
+    ∃ (Ls : List (Option (List α))) (L : List α), models A Ls L := by -/
 
-    done
-  stop
-  done
+/- theorem exists_model' (Ls : List (Option (List α))) (L : List α) :
+    ∃ (A : RangeArray α), models A Ls L := by -/
 
 /-! # fold -/
 
@@ -1170,13 +1184,17 @@ def foldl_index {β : Type v} (f : β → α → β)
 
 @[inline, always_inline, specialize]
 def foldlM_indexHyps {β : Type v} {m : Type v → Type w} [Monad m] (f : β → α → m β)
-    (init : β) (A : RangeArray α) (i : Fin A.size) (h_del : A.isDeletedFin i = false) : m β :=
-  A.data.foldlM f init (A.indexFin i) (A.indexFin i + A.rsizeFin i)
+    (init : β) (A : RangeArray α) (i : Fin A.size) : m β :=
+  if isDeleted A i = false then
+    A.data.foldlM f init (A.indexFin i) (A.indexFin i + A.rsizeFin i)
+  else return init
 
 @[inline, always_inline, specialize]
 def foldl_indexHyps {β : Type v} (f : β → α → β)
-    (init : β) (A : RangeArray α) (i : Fin A.size) (h_del : A.isDeletedFin i = false) : β :=
-  A.data.foldl f init (A.indexFin i) (A.indexFin i + A.rsizeFin i)
+    (init : β) (A : RangeArray α) (i : Fin A.size) : β :=
+  if isDeleted A i = false then
+    A.data.foldl f init (A.indexFin i) (A.indexFin i + A.rsizeFin i)
+  else init
 
 @[inline, always_inline, specialize]
 def ufoldlM {β : Type v} {m : Type v → Type w} [Monad m] (f : β → α → m β)
@@ -1199,13 +1217,10 @@ theorem unitProp.go.cons_aux (τ : PPA) (l : ILit) {ls : List ILit} {i j : Nat} 
 
 #check LeanColls.Seq
 #check Option.bind
-theorem foldlM_index_eq_foldlM {A : RangeArray α} {Ls : List (Option (List α))} {L : List α}
-    (h_models : models A Ls L)
-    {i : Nat} {hi : i < Size.size Ls}
+theorem foldlM_index_eq_foldlM {i : Nat} {hi : i < Size.size Ls}
     {sL : List α} (hsL : Seq.get Ls ⟨i, hi⟩ = some sL)
     {β : Type v} {m : Type v → Type w} [Monad m] (f : β → α → m β) (init : β) :
-    A.foldlM_index f init i =
-      sL.foldlM f init := by
+    R.foldlM_index f init i = sL.foldlM f init := by
   rw [foldlM_index]
   have := h_models.h_some hi
   simp [hsL] at this
@@ -1221,67 +1236,6 @@ theorem foldlM_index_eq_foldlM {A : RangeArray α} {Ls : List (Option (List α))
   done
 
 #exit
-
--- Kind of like a Seq
-class RangeArrayApi (C : Type _) where
-  size : C → Nat
-  rsize : (cont : C) → (i : Fin (size cont)) → Nat
-  get : (cont : C) → (i : Fin (size cont)) → (offset : Fin (rsize cont i)) → α
-  isDeleted : C → Nat → Bool
-  foldlM {β : Type v} {m : Type v → Type w} [Monad m] :
-    (f : β → α → m β) → (init : β)
-      → (cont : C) → (i : Nat) → m β
-  foldl {β : Type v} :
-    (f : β → α → β) → (init : β)
-      → (cont : C) → (i : Nat) → β
-      --fun f init cont i hi =>
-      --  Id.run <| @foldlM β Id _ f init cont i hi
-
-
-
-#exit
-
-theorem models_add_of_empty : models R as #[] → ∀ (arr : Array α), models (R.add arr) (as.push arr) #[] := by
-  intro h_models arr
-  convert models_add h_models arr
-  exact (nil_append arr).symm
-
-
-
---theorem fn_eq_of_models : models R as c → ∀ (f : Nat → α)
-
-#exit
-
-theorem index_OoB {A : RangeArray α} {i : Nat} : i ≥ A.size → A.index i = 0 := by
-  simp [index]
-  intro h hcon
-  exact absurd hcon (not_lt_of_ge h)
-
-theorem rsize_OoB {A : RangeArray α} {i : Nat} : i ≥ A.size → A.rsize i = 0 := by
-  simp [rsize]
-  intro h
-  have := le_trans h (le_succ _)
-  simp [index_OoB h, index_OoB this]
-  rintro _ heq
-  simp [← heq] at h
-
-theorem index_add_rsize_of_lt {A : RangeArray α} {i : Nat} :
-    i + 1 < A.size → A.index i + A.rsize i = A.index (i + 1) := by
-  intro hi
-  simp [index, rsize, hi, lt_of_succ_lt hi, -get_eq_getElem]
-  rw [← Nat.add_sub_assoc, Nat.add_comm, Nat.add_sub_cancel]
-  exact A.h_indexes_inc i hi
-
-theorem index_add_rsize_of_eq {A : RangeArray α} {i : Nat} :
-    i + 1 = A.size → A.index i + A.rsize i = A.dsize := by
-  intro hi
-  have hi' := lt_of_succ_le (le_of_eq hi)
-  simp [index, rsize, hi, hi', -get_eq_getElem]
-  rw [← Nat.add_sub_assoc, Nat.add_comm, Nat.add_sub_cancel]
-  exact A.h_indexes ⟨i, hi'⟩
-
-/-! # fold -/
-
 
 
 @[simp]
@@ -1399,484 +1353,5 @@ theorem foldl_add {β : Type v} (g : β → α → β) (f : β → β → β)
   --exact foldlM_add (m := Id) g f initg initf _ _
   sorry
   done
-
-/-! # model -/
-
-def subArray (i : Nat) : Array α :=
-  A.foldl_index Array.push #[] i
-
-#check foldlM.loop
-#check Nat.lt_trichotomy
-
-theorem foldlM_eq_subArray_foldlM {β : Type v} {m : Type v → Type w} [Monad m]
-    (f : β → α → m β) (init : β) (i : Nat) :
-      A.foldlM_index f init i = (A.subArray i).foldlM f init := by
-  simp [subArray, foldlM_index]
-  generalize h_range : A.rsize i = range
-  induction range using Nat.recAux generalizing i with
-  | zero => simp [foldl_index_trivial h_range]
-  | succ range ih =>
-    sorry
-    done
-
-end RangeArray
-
-----------------------------------
-
-namespace LeanSAT
-
-open LeanSAT LeanSAT.Model PropFun
-
-open RangeArray
-
-instance : ToString (RangeArray ILit) where
-  toString F := F.foldl (· ++ s!" {·}") (· ++ "\n" ++ ·) "" ""
-
-def toPropFun (F : RangeArray ILit) : PropFun IVar :=
-    F.foldl (· ⊔ ·.toPropFun) (· ⊓ ·) ⊥ ⊤
-
-@[simp]
-theorem toPropFun_empty : toPropFun (RangeArray.empty : RangeArray ILit) = ⊤ := by
-  simp [toPropFun]
-
-theorem toPropFun_add (RA : RangeArray ILit) (C : IClause) :
-    toPropFun (RA.add C) = (toPropFun RA) ⊓ C.toPropFun := by
-  simp_rw [toPropFun]
-  rw [foldl_add, Clause.foldl_bot_toPropFun_eq]
-
-end LeanSAT
-
-#exit
-
-/-
-/-! ### extract -/
-
-theorem extract_loop_zero (as bs : Array α) (start : Nat) : extract.loop as 0 start bs = bs := by
-  rw [extract.loop]; split <;> rfl
-
-theorem extract_loop_succ (as bs : Array α) (size start : Nat) (h : start < as.size) :
-    extract.loop as (size+1) start bs = extract.loop as size (start+1) (bs.push as[start]) := by
-  rw [extract.loop, dif_pos h]; rfl
-
-theorem extract_loop_of_ge (as bs : Array α) (size start : Nat) (h : start ≥ as.size) :
-    extract.loop as size start bs = bs := by
-  rw [extract.loop, dif_neg (Nat.not_lt_of_ge h)]
-
-theorem extract_loop_eq_aux (as bs : Array α) (size start : Nat) :
-    extract.loop as size start bs = bs ++ extract.loop as size start #[] := by
-  induction size using Nat.recAux generalizing start bs with
-  | zero => rw [extract_loop_zero, extract_loop_zero, append_nil]
-  | succ size ih =>
-    if h : start < as.size then
-      rw [extract_loop_succ (h:=h), ih (bs.push _), push_eq_append_singleton]
-      rw [extract_loop_succ (h:=h), ih (#[].push _), push_eq_append_singleton, nil_append]
-      rw [append_assoc]
-    else
-      rw [extract_loop_of_ge (h:=Nat.le_of_not_lt h)]
-      rw [extract_loop_of_ge (h:=Nat.le_of_not_lt h)]
-      rw [append_nil]
-
-theorem extract_loop_eq (as bs : Array α) (size start : Nat) (h : start + size ≤ as.size) :
-  extract.loop as size start bs = bs ++ as.extract start (start + size) := by
-  simp [extract]; rw [extract_loop_eq_aux, Nat.min_eq_left h, Nat.add_sub_cancel_left]
--/
-
-theorem rsize_lt_size (i : Fin A.size) : A.rsize i ≤ A.dsize - A.index i := by
-  simp [index, rsize]
-  by_cases h_index : i.val + 1 < A.size <;> simp [h_index]
-  rw [Nat.sub_add_cancel]
-  exact A.h_indexes ⟨i.val + 1, h_index⟩
-  exact A.h_indexes i
-
-def get (i : Fin A.size) (j : Fin (A.rsize i)) : α :=
-  A.data.get ⟨A.index i, by
-    rcases i with ⟨i, hi⟩
-    rcases j with ⟨j, hj⟩
-    have := A.h_indexes ⟨i, hi⟩
-    rcases eq_or_lt_of_le this with (hi_eq | hi_lt)
-    · have h : A.dsize - A.index ⟨i, hi⟩ = 0 := by
-        exact (Nat.sub_eq_iff_eq_add' this).mpr (id hi_eq.symm)
-      have := rsize_lt_size _ ⟨i, hi⟩
-      rw [h, le_zero] at this
-      rw [this] at hj
-      contradiction
-    · exact hi_lt⟩
-
-def delete (i : Fin A.size) : RangeArray α := { A with
-  deleted := A.deleted.set ⟨i, by rw [← A.h_sizes_eq]; exact i.isLt⟩ true
-  deletedSize := A.deletedSize + A.rsize i
-  h_sizes_eq := by simp [A.h_sizes_eq]
-}
-
-def isDeleted (i : Fin A.size) : Bool := A.deleted.get ⟨i, by rw [← A.h_sizes_eq]; exact i.isLt⟩
-
-@[simp] theorem size_empty : (empty : RangeArray α).size = 1 := by simp [empty, size]
-@[simp] theorem dsize_empty : (empty : RangeArray α).dsize = 0 := by simp [empty, dsize]; rfl
-@[simp] theorem rsize_empty : (empty : RangeArray α).rsize ⟨0, by simp⟩ = 0 := by simp [empty]; rfl
-@[simp] theorem size_push : (A.push v).size = A.size := by simp [push, size]
-@[simp] theorem dsize_push : (A.push v).dsize = A.dsize + 1 := by simp [push, dsize]
-
-@[simp]
-theorem rsize_push (i : Fin A.size) : (A.push v).rsize i =
-    if i.val + 1 = A.size then A.rsize i + 1 else A.rsize i := by
-  simp [push, rsize]
-  rcases i with ⟨i, hi⟩
-  by_cases h_index : i + 1 < A.size
-  · simp [h_index, Nat.ne_of_lt h_index]; rfl
-  · simp [h_index]
-    simp at h_index
-    simp [le_antisymm h_index (succ_le_of_lt hi), index]
-    rw [Nat.sub_add_comm]
-    exact A.h_indexes _
-
-@[simp] theorem size_cap : (A.cap).size = A.size + 1 := by simp [cap, size]
-@[simp] theorem dsize_cap : (A.cap).dsize = A.dsize := by simp [cap, dsize]
-
-@[simp]
-theorem rsize_cap (i : Fin A.size) : (A.cap).rsize ⟨i.val, by rw [size_cap]; exact lt_succ_of_lt i.isLt⟩ = A.rsize i := by
-  simp [cap, rsize, index]; sorry
-
-@[simp] theorem size_delete (i : Fin A.size) : (A.delete i).size = A.size := by simp [delete, size]
-@[simp] theorem dsize_delete (i : Fin A.size) : (A.delete i).dsize = A.dsize := by simp [delete, dsize]
-
-@[simp]
-theorem rsize_delete (i j : Fin A.size) : (A.delete i).rsize j =
-    if i.val = j.val then 0 else A.rsize j := by
-  simp [delete, rsize]; sorry
-
-def zeroFin : Fin A.size := ⟨0, A.h_indexes_size_pos⟩
-def predFin : Fin A.size := ⟨A.size - 1, by
-    match hA' : A.size with
-    | 0 => have hA := A.h_indexes_size_pos; simp [hA'] at hA; | n + 1 => simp⟩
-
-@[inline, specialize]
-def foldlM_index {β : Type v} {m : Type v → Type w} [Monad m] (f : β → α → m β)
-    (init : β) (A : RangeArray α) (i : Fin A.size) : m β :=
-  A.data.foldlM f init (A.index i) (A.index i + A.rsize i)
-
-@[inline]
-def foldl_index {β : Type v} (f : β → α → β)
-    (init : β) (A : RangeArray α) (i : Fin A.size) : β :=
-  Id.run <| A.foldlM_index f init i
-
-@[simp]
-theorem foldlM_index_empty {β : Type v} {m : Type v → Type w} [Monad m]
-    (f : β → α → m β) (init : β) (i : Fin empty.size) :
-      (empty : RangeArray α).foldlM_index f init i = return init := by
-  simp [foldlM_index, empty, foldlM]
-  rcases i with ⟨i, hi⟩
-  simp at hi
-  subst hi
-  simp
-  sorry
-
-@[simp]
-theorem foldl_index_empty {β : Type v} (f : β → α → β) (init : β) (i : Fin empty.size) :
-      (empty : RangeArray α).foldl_index f init i = init := by
-  simp [foldl_index, empty, foldlM_index_empty]
-  sorry
-
-theorem foldl_index_push_lt {β : Type v} (f : β → α → β) (init : β) (i : Fin A.size) (h : i.val + 1 < A.size) :
-    (A.push v).foldl_index f init i = A.foldl_index f init i := by
-  simp [foldl_index, push, foldlM_index]
-  sorry
-
-theorem foldl_index_push_eq {β : Type v} (f : β → α → β) (init : β) (i : Fin A.size) (h : i.val + 1 = A.size) :
-    (A.push v).foldl_index f init i = f init v := by
-  simp [foldl_index, push, foldlM_index]
-  sorry
-
-/-
-@[inline, specialize]
-def foldlM {α : Type u} {β : Type v} {γ : Type w} {m₁ : Type v → Type w} {m₂ : Type w → Type x}
-    [Monad m₁] [Monad m₂] (f_inner : β → α → m₁ β) (f_outer : γ → β → m₂ γ)
-    (init_inner : β) (init_outer : γ) (A : RangeArray α) (start stop : Fin A.size) : m₂ γ := -/
-
-@[inline, specialize]
-def foldlM {α : Type u} {β : Type v} {m : Type v → Type w}
-    [Monad m] (f_inner : β → α → m β) (f_outer : β → β → m β)
-    (init_inner init_outer : β) (A : RangeArray α)
-    (start : Fin A.size := A.zeroFin)
-    (stop : Fin A.size := A.predFin) : m β :=
-  Fin.foldRangeM (fun i b => do
-    if !A.isDeleted i then
-      f_outer b (← A.foldlM_index f_inner init_inner i)
-    else
-      return b) init_outer start stop
-
-@[inline]
-def foldl {α : Type u} {β : Type v} (f_inner : β → α → β) (f_outer : β → β → β)
-    (init_inner init_outer : β) (A : RangeArray α)
-      (start : Fin A.size := A.zeroFin)
-      (stop : Fin A.size := A.predFin) : β :=
-  Fin.foldRange (fun i b => f_outer b (A.foldl_index f_inner init_inner i)) init_outer start stop
-
-@[simp]
-theorem foldl_empty {α : Type u} {β : Type v} (f_inner : β → α → β) (f_outer : β → β → β)
-    (init_inner init_outer : β) (start stop : Fin empty.size) :
-      (empty : RangeArray α).foldl f_inner f_outer init_inner init_outer start stop = init_outer := by
-  rcases start with ⟨start, hstart⟩
-  rcases stop with ⟨stop, hstop⟩
-  simp at hstart hstop
-  simp [foldl, hstart, hstop]
-
-structure models (RA : RangeArray α) (A : Array (Array α)) : Prop :=
-  (h_outer_size : RA.size = A.size)
-  (h_inner_size : ∀ (i : Fin RA.size), RA.rsize i = Array.size (A.get ⟨i.val, by
-      have := i.isLt; simp [h_outer_size] at this; exact this⟩))
-  (h_data : ∀ (i : Fin RA.size) (j : Fin (RA.rsize i)), RA.get i j = (A.get ⟨i.val, by
-      have := i.isLt; simp [h_outer_size] at this; exact this⟩).get ⟨j.val, by
-        have := j.isLt; simp [h_inner_size] at this; exact this⟩)
-
-instance [ToString α] : ToString (RangeArray α) where
-  toString A := A.foldl (· ++ s!" {·}") (· ++ "\n" ++ ·) "" ""
-
-end RangeArray
-
-open LeanSAT LeanSAT.Model PropFun
-
-abbrev FlatCnf := RangeArray ILit
-
-namespace FlatCnf
-
-open RangeArray
-
-instance : ToString FlatCnf where
-  toString F := F.foldl (· ++ s!" {·}") (· ++ "\n" ++ ·) "" ""
-
-def toPropFun (F : FlatCnf) : PropFun IVar :=
-    F.foldl (· ⊔ ·.toPropFun) (· ⊓ ·) ⊥ ⊤
-      ⟨0, F.h_indexes_size_pos⟩ ⟨F.size - 1, by
-        match hF' : F.size with
-        | 0 =>
-          have hF := F.h_indexes_size_pos
-          simp [hF'] at hF
-        | n + 1 => simp⟩
-
-def backToPropFun (F : FlatCnf) : PropFun IVar :=
-  F.foldl_index (· ⊔ ·.toPropFun) ⊥ ⟨F.size - 1, by
-    match hF' : F.size with
-    | 0 =>
-      have hF := F.h_indexes_size_pos
-      simp [hF'] at hF
-    | n + 1 => simp⟩
-
-@[simp]
-theorem toPropFun_empty : toPropFun (RangeArray.empty : FlatCnf) = ⊤ := by
-  simp [toPropFun]
-
-@[simp]
-theorem backToPropFun_empty : backToPropFun (RangeArray.empty : FlatCnf) = ⊥ := by
-  simp [backToPropFun]
-
-variable (F : FlatCnf) (l : ILit)
-
-@[simp]
-theorem backToPropFun_push : backToPropFun (push F l) = F.backToPropFun ⊔ l.toPropFun := by
-  simp [backToPropFun, push, Id.run]
-  sorry
-  done
-
-end FlatCnf
-
-
-#exit
-def get  (i : Fin A.data.size) : α := A.data.get i
-def get? (i : Nat) : Option α := A.data.get? i
-def get! [Inhabited α] (A : RangeArray α) (i : Nat) : α := A.data.get! i
-
-def set (i : Fin A.data.size) (v : α) : RangeArray α := { A with
-  data := A.data.set i v
-  h_indexes := by rw [size_set]; exact A.h_indexes
-}
-
-def set! (i : Nat) (v : α) : RangeArray α := { A with
-  data := A.data.set! i v
-  h_indexes := by rw [size_set!]; exact A.h_indexes
-}
-
-def range (index : Fin A.indexes.size) : Nat × Nat :=
-  if hi : index.val + 1 = A.indexes.size then
-    ⟨A.indexes.get index, A.data.size⟩
-  else
-    ⟨A.indexes.get index, A.indexes.get ⟨index.val + 1, Fin.succFin_of_ne hi⟩⟩
-
-def range! (index : Nat) : Nat × Nat :=
-  if hi : index < A.indexes.size then
-    A.range ⟨index, hi⟩
-  else
-    ⟨0, 0⟩
-
-def backRange : Nat × Nat :=
-  if A.indexes.back = A.data.size then
-    if A.indexes.size < 2 then
-      ⟨0, 0⟩
-    else
-      ⟨A.indexes.get! (A.indexes.size - 2), A.indexes.get! (A.indexes.size - 1)⟩
-  else
-    ⟨A.indexes.back, A.data.size⟩
-
-def sizeAt (index : Fin A.indexes.size) : Nat :=
-  let ⟨s, e⟩ := A.range index
-  e - s
-
-def sizeAt! (index : Nat) : Nat :=
-  let ⟨s, e⟩ := A.range! index
-  e - s
-
-def getAt (index : Fin A.indexes.size) (i : Fin (A.sizeAt index)) : α :=
-  A.get ⟨(A.indexes.get index) + i.val, by
-    have ⟨i, hi⟩ := i
-    simp [sizeAt, range] at hi
-    by_cases h_index : index.val + 1 = A.indexes.size
-    · simp [h_index] at hi
-      have := Nat.add_lt_add_right hi (CArray.get A.indexes index)
-      rw [Nat.sub_add_cancel (le_of_lt_succ (A.h_indexes index))] at this
-      rw [add_comm]
-      exact this
-    · simp [h_index] at hi
-      simp only [gt_iff_lt]
-      have := Nat.add_lt_add_right hi (CArray.get A.indexes index)
-      rw [Nat.sub_add_cancel] at this
-      rw [add_comm]
-      exact lt_of_lt_of_le this (le_of_lt_succ (A.h_indexes ⟨index.val + 1, _⟩))
-      · apply Nat.not_lt.mp
-        intro h_contra
-        rw [Nat.sub_eq_zero_of_le (le_of_lt h_contra)] at hi
-        contradiction⟩
-
-def getAt! [Inhabited α] (index i : Nat) : α :=
-  A.get! ((A.indexes.get! index) + i)
-
-/-! # fold -/
-
-@[inline]
-def foldlMAtIndex {α : Type u} {β : Type v} {m : Type v → Type w} [Monad m] (f : β → α → m β) (init : β) (A : RangeArray α) (index : Nat) : m β :=
-  let ⟨s, e⟩ := A.range! index
-  A.data.foldlM f init s e
-
-@[inline]
-def foldrMAtIndex {α : Type u} {β : Type v} {m : Type v → Type w} [Monad m] (f : α → β → m β) (init : β) (A : RangeArray α) (index : Nat) : m β :=
-  let ⟨s, e⟩ := A.range! index
-  A.data.foldrM f init s e
-
-@[inline]
-def foldlAtIndex {α : Type u} {β : Type v} (f : β → α → β) (init : β) (A : RangeArray α) (index : Nat) : β :=
-  Id.run <| A.foldlMAtIndex f init index
-
-@[inline]
-def foldrAtIndex {α : Type u} {β : Type v} (f : α → β → β) (init : β) (A : RangeArray α) (index : Nat) : β :=
-  Id.run <| A.foldrMAtIndex f init index
-
-@[inline]
-def foldlMOverIndices {β : Type v} {m : Type v → Type w} [Monad m] (f : β → Nat → m β) (init : β) (A : RangeArray α) (start := 0) (stop := A.indexes.size) :=
-  A.indexes.foldlM f init start stop
-
-@[inline]
-def foldrMOverIndices {β : Type v} {m : Type v → Type w} [Monad m] (f : Nat → β → m β) (init : β) (A : RangeArray α) (start := 0) (stop := A.indexes.size) :=
-  A.indexes.foldrM f init start stop
-
-@[inline]
-def foldlOverIndices {β : Type v} (f : β → Nat → β) (init : β) (A : RangeArray α) (start := 0) (stop := A.indexes.size) :=
-  Id.run <| A.foldlMOverIndices f init start stop
-
-@[inline]
-def foldrOverIndices {β : Type v} (f : Nat → β → β) (init : β) (A : RangeArray α) (start := 0) (stop := A.indexes.size) :=
-  Id.run <| A.foldrMOverIndices f init start stop
-
-/-! # fold behavior -/
-
-/- The goal is to prove that the RangeArray acts like an array of arrays. -/
-
-/-
-section fromArrays
-
-variable (as : Array (Array α)) (RA : RangeArray α)
-
-def fromArrays : RangeArray α :=
-  as.foldl (fun RA a => (a.foldl (fun RA x => RA.push x) RA).cap) (RangeArray.empty)
-
-@[simp]
-theorem fromArrays_empty : (fromArrays (#[] : Array (Array α))) = RangeArray.empty := by
-  simp [fromArrays, empty, foldl]
-
-@[simp]
-theorem fromArrays_nil : (fromArrays ({ data := [] } : Array (Array α))) = RangeArray.empty := by
-  simp [fromArrays, empty, foldl]
-
-@[simp]
-theorem foldlM_eq {α : Type u} {β : Type v} {m : Type v → Type w} [Monad m]
-    (f : β → α → m β) (init : β) (as : Array (Array α))
-      (index : Nat) (h_index : index < as.size) :
-    (fromArrays as).foldlMAtIndex f init index = (as.get ⟨index, h_index⟩).foldlM f init := by
-  have ⟨as⟩ := as
-  rw [foldlMAtIndex]
-  induction' as with A AS ih generalizing index
-  · simp at h_index
-  · match index with
-    | 0 =>
-      simp [fromArrays, Array.foldl_eq_foldl_data]
-      done
-    done
-  done
-  -/
-
-
-
-def toPropFun (A : RangeArray ILit) : PropFun IVar :=
-  Fin.foldl A.numPartitions (fun F index =>
-    A.foldlAtIndex)
-  --sorry
-
-#exit
-
-@[simp] theorem size_fromArrays : (fromArrays as).size = as.size := by sorry
-  /-rcases as with ⟨as⟩
-  induction' as with B BS ih
-  · simp [fromArrays]; rfl
-  ·
-    done
-  simp [fromArrays]
-  done -/
-
--- def getAt (index : Fin A.indexes.size) (i : Fin (A.sizeAt index))
-theorem fromArrays_foldl {β : Type v} (as : Array (Array α)) (index : Fin as.size)
-    (f : β → α → β) (init : β) :
-    (as.get index).foldl f init = (fromArrays as).foldlAtIndex f init index.val := by
-  sorry
-  done
-
-
-end fromArrays
-
-instance [ToString α] : ToString (RangeArray α) where
-  toString a := s!"({a.data}, {a.indexes})"
-
-/-- Creates a new container that contains any elements added via `push`,
-    but that container is marked as deleted. -/
-/-
-def commitDeleted : RangeArray α := { A with
-  indexes := A.indexes.push (markIndexAsDeleted A.dsize)
-  dataSize := A.data.size
-  h_size := le.refl
-  h_indexes := by
-    intro i hi
-    simp at hi
-    rcases eq_or_lt_of_le (le_of_lt_succ hi) with (rfl | hi)
-    · simp [get_push, -markIndexAsDeleted_coe]
-      exact A.h_size
-    · simp [get_push, hi]
-      exact le_trans (A.h_indexes hi) A.h_size
-  h_indexes_inc := by
-    intro i hi
-    simp at hi
-    simp [get_push, hi, -markIndexAsDeleted_coe]
-    rcases eq_or_lt_of_le (succ_le_of_lt hi) with (hi' | hi')
-    · rw [succ_eq_add_one] at hi'
-      simp [hi', -markIndexAsDeleted_coe]
-      exact A.h_indexes _
-    · simp [hi']
-      exact A.h_indexes_inc hi'
-} -/
 
 end RangeArray
